.lake/build/ir/IVI/Demo.c
@@ -60,7 +60,7 @@ lean_object* l_Nat_reprFast(lean_object*);
 static lean_object* l_main___closed__16;
 static double l_main___closed__11;
 double l_IVI_graininessScore(lean_object*);
-LEAN_EXPORT lean_object* l_main___lam__5(double, double, double, lean_object*, lean_object*, lean_object*, lean_object*, lean_object*, lean_object*, lean_object*, lean_object*, double, double, double, lean_object*);
+LEAN_EXPORT lean_object* l_main___lam__5(lean_object*, uint8_t, lean_object*, lean_object*, double, double, double, lean_object*, lean_object*, lean_object*, lean_object*, lean_object*, lean_object*, lean_object*, double, double, double, lean_object*);
 static lean_object* l_main___closed__53;
 static lean_object* l_main___closed__47;
 static double l_main___closed__58;
@@ -132,7 +132,7 @@ LEAN_EXPORT lean_object* l_IO_print___at___IO_println___at___main_logZooms_spec_
 static lean_object* l_main_logZooms___closed__12;
 lean_object* l_IVI_Invariant_runUntilConverged(lean_object*, lean_object*, lean_object*, lean_object*);
 static lean_object* l_List_toString___at___main_spec__14___closed__1;
-LEAN_EXPORT lean_object* l_main___lam__5___boxed(lean_object*, lean_object*, lean_object*, lean_object*, lean_object*, lean_object*, lean_object*, lean_object*, lean_object*, lean_object*, lean_object*, lean_object*, lean_object*, lean_object*, lean_object*);
+LEAN_EXPORT lean_object* l_main___lam__5___boxed(lean_object**);
 uint8_t lean_nat_dec_eq(lean_object*, lean_object*);
 lean_object* l_IVI_ITranslation_zoomE(lean_object*, lean_object*);
 lean_object* lean_float_to_string(double);
@@ -413,314 +413,318 @@ x_20 = l_IVI_KakeyaField_collapseScore(x_19);
 x_21 = l_IVI_KakeyaField_collapseExceededBool(x_19);
 if (x_21 == 0)
 {
-lean_object* x_22; lean_object* x_23; lean_object* x_24; lean_object* x_25; lean_object* x_26; lean_object* x_27; lean_object* x_28; lean_object* x_29; lean_object* x_35; uint8_t x_36; lean_object* x_37; lean_object* x_38; lean_object* x_45; uint8_t x_46; uint8_t x_47; lean_object* x_48; lean_object* x_49; lean_object* x_56; uint8_t x_57; uint8_t x_58; lean_object* x_59; uint8_t x_60; lean_object* x_61; lean_object* x_68; lean_object* x_69; double x_70; double x_71; lean_object* x_72; lean_object* x_73; lean_object* x_74; double x_75; uint8_t x_76; uint8_t x_77; uint8_t x_78; lean_object* x_79; uint8_t x_80; uint8_t x_81; lean_object* x_82; lean_object* x_83; uint8_t x_90; uint8_t x_91; uint8_t x_92; uint8_t x_121; uint8_t x_126; 
+lean_object* x_22; lean_object* x_23; lean_object* x_24; lean_object* x_25; double x_26; lean_object* x_27; lean_object* x_28; lean_object* x_29; lean_object* x_30; lean_object* x_31; uint8_t x_37; lean_object* x_38; lean_object* x_39; lean_object* x_40; uint8_t x_47; lean_object* x_48; uint8_t x_49; lean_object* x_50; lean_object* x_51; uint8_t x_58; uint8_t x_59; lean_object* x_60; uint8_t x_61; lean_object* x_62; lean_object* x_63; lean_object* x_70; lean_object* x_71; double x_72; double x_73; lean_object* x_74; lean_object* x_75; lean_object* x_76; double x_77; uint8_t x_78; uint8_t x_79; uint8_t x_80; uint8_t x_81; lean_object* x_82; uint8_t x_83; lean_object* x_84; lean_object* x_85; uint8_t x_92; uint8_t x_93; uint8_t x_94; uint8_t x_123; uint8_t x_128; 
 lean_inc(x_1);
 x_22 = l_IVI_ITranslation_zoomE(x_1, x_9);
 x_23 = lean_ctor_get(x_22, 0);
 lean_inc(x_23);
 lean_dec(x_22);
-x_24 = lean_ctor_get(x_23, 1);
+x_24 = lean_ctor_get(x_6, 0);
 lean_inc(x_24);
-x_25 = lean_unsigned_to_nat(1u);
-x_26 = lean_nat_sub(x_7, x_25);
+x_25 = lean_ctor_get(x_23, 1);
+lean_inc(x_25);
+x_26 = lean_ctor_get_float(x_24, sizeof(void*)*1);
+lean_dec(x_24);
+x_27 = lean_unsigned_to_nat(1u);
+x_28 = lean_nat_sub(x_7, x_27);
 lean_dec(x_7);
-x_68 = lean_box(1);
-x_69 = l_IVI_Invariant_resonanceMatrixW(x_16, x_24);
-lean_inc(x_69);
-x_70 = l_IVI_graininessScore(x_69);
-x_71 = l_main_logZooms___closed__6;
-x_72 = l_main_logZooms___boxed__const__1;
-x_73 = l_main_logZooms___boxed__const__2;
+x_70 = lean_box(1);
+x_71 = l_IVI_Invariant_resonanceMatrixW(x_16, x_25);
+lean_inc(x_71);
+x_72 = l_IVI_graininessScore(x_71);
+x_73 = l_main_logZooms___closed__6;
+x_74 = l_main_logZooms___boxed__const__1;
+x_75 = l_main_logZooms___boxed__const__2;
 lean_inc(x_5);
-x_74 = lean_apply_4(x_5, x_17, x_69, x_72, x_73);
-x_75 = lean_unbox_float(x_74);
-lean_dec(x_74);
-x_76 = lean_float_decLe(x_70, x_3);
-x_77 = lean_float_decLe(x_4, x_75);
-x_126 = lean_float_decLe(x_20, x_2);
-if (x_126 == 0)
+x_76 = lean_apply_4(x_5, x_17, x_71, x_74, x_75);
+x_77 = lean_unbox_float(x_76);
+lean_dec(x_76);
+x_78 = lean_float_decLe(x_72, x_3);
+x_79 = lean_float_decLe(x_4, x_77);
+x_128 = lean_float_decLe(x_20, x_26);
+if (x_128 == 0)
 {
-x_121 = x_21;
-goto block_125;
+x_123 = x_21;
+goto block_127;
 }
 else
 {
-uint8_t x_127; 
-x_127 = lean_unbox(x_68);
-x_121 = x_127;
-goto block_125;
+uint8_t x_129; 
+x_129 = lean_unbox(x_70);
+x_123 = x_129;
+goto block_127;
 }
-block_34:
+block_36:
 {
-lean_object* x_30; lean_object* x_31; 
-x_30 = lean_string_append(x_27, x_29);
-lean_dec(x_29);
-x_31 = l_IO_println___at___main_logZooms_spec__0(x_30, x_10);
-if (lean_obj_tag(x_31) == 0)
-{
-lean_object* x_32; 
-x_32 = lean_ctor_get(x_31, 1);
-lean_inc(x_32);
+lean_object* x_32; lean_object* x_33; 
+x_32 = lean_string_append(x_29, x_31);
 lean_dec(x_31);
-x_7 = x_26;
-x_8 = x_28;
+x_33 = l_IO_println___at___main_logZooms_spec__0(x_32, x_10);
+if (lean_obj_tag(x_33) == 0)
+{
+lean_object* x_34; 
+x_34 = lean_ctor_get(x_33, 1);
+lean_inc(x_34);
+lean_dec(x_33);
+x_7 = x_28;
+x_8 = x_30;
 x_9 = x_23;
-x_10 = x_32;
+x_10 = x_34;
 goto _start;
 }
 else
 {
+lean_dec(x_30);
 lean_dec(x_28);
-lean_dec(x_26);
 lean_dec(x_23);
 lean_dec(x_6);
 lean_dec(x_5);
 lean_dec(x_1);
-return x_31;
+return x_33;
 }
 }
-block_44:
+block_46:
 {
-lean_object* x_39; lean_object* x_40; lean_object* x_41; 
-x_39 = lean_string_append(x_35, x_38);
-lean_dec(x_38);
-x_40 = l_main_logZooms___closed__0;
-x_41 = lean_string_append(x_39, x_40);
-if (x_36 == 0)
+lean_object* x_41; lean_object* x_42; lean_object* x_43; 
+x_41 = lean_string_append(x_38, x_40);
+lean_dec(x_40);
+x_42 = l_main_logZooms___closed__0;
+x_43 = lean_string_append(x_41, x_42);
+if (x_37 == 0)
 {
-lean_object* x_42; 
-x_42 = l_main_logZooms___closed__1;
-x_27 = x_41;
-x_28 = x_37;
-x_29 = x_42;
-goto block_34;
-}
-else
-{
-lean_object* x_43; 
-x_43 = l_main_logZooms___closed__2;
-x_27 = x_41;
-x_28 = x_37;
+lean_object* x_44; 
+x_44 = l_main_logZooms___closed__1;
 x_29 = x_43;
-goto block_34;
-}
-}
-block_55:
-{
-lean_object* x_50; lean_object* x_51; lean_object* x_52; 
-x_50 = lean_string_append(x_45, x_49);
-lean_dec(x_49);
-x_51 = l_main_logZooms___closed__3;
-x_52 = lean_string_append(x_50, x_51);
-if (x_47 == 0)
-{
-lean_object* x_53; 
-x_53 = l_main_logZooms___closed__1;
-x_35 = x_52;
-x_36 = x_46;
-x_37 = x_48;
-x_38 = x_53;
-goto block_44;
+x_30 = x_39;
+x_31 = x_44;
+goto block_36;
 }
 else
 {
-lean_object* x_54; 
-x_54 = l_main_logZooms___closed__2;
-x_35 = x_52;
-x_36 = x_46;
-x_37 = x_48;
+lean_object* x_45; 
+x_45 = l_main_logZooms___closed__2;
+x_29 = x_43;
+x_30 = x_39;
+x_31 = x_45;
+goto block_36;
+}
+}
+block_57:
+{
+lean_object* x_52; lean_object* x_53; lean_object* x_54; 
+x_52 = lean_string_append(x_48, x_51);
+lean_dec(x_51);
+x_53 = l_main_logZooms___closed__3;
+x_54 = lean_string_append(x_52, x_53);
+if (x_49 == 0)
+{
+lean_object* x_55; 
+x_55 = l_main_logZooms___closed__1;
+x_37 = x_47;
 x_38 = x_54;
-goto block_44;
-}
-}
-block_67:
-{
-lean_object* x_62; lean_object* x_63; lean_object* x_64; 
-x_62 = lean_string_append(x_56, x_61);
-lean_dec(x_61);
-x_63 = l_main_logZooms___closed__4;
-x_64 = lean_string_append(x_62, x_63);
-if (x_57 == 0)
-{
-lean_object* x_65; 
-x_65 = l_main_logZooms___closed__1;
-x_45 = x_64;
-x_46 = x_58;
-x_47 = x_60;
-x_48 = x_59;
-x_49 = x_65;
-goto block_55;
+x_39 = x_50;
+x_40 = x_55;
+goto block_46;
 }
 else
 {
-lean_object* x_66; 
-x_66 = l_main_logZooms___closed__2;
-x_45 = x_64;
-x_46 = x_58;
-x_47 = x_60;
-x_48 = x_59;
-x_49 = x_66;
-goto block_55;
+lean_object* x_56; 
+x_56 = l_main_logZooms___closed__2;
+x_37 = x_47;
+x_38 = x_54;
+x_39 = x_50;
+x_40 = x_56;
+goto block_46;
 }
 }
-block_89:
+block_69:
 {
-lean_object* x_84; lean_object* x_85; lean_object* x_86; 
-x_84 = lean_string_append(x_79, x_83);
-lean_dec(x_83);
-x_85 = l_main_logZooms___closed__7;
-x_86 = lean_string_append(x_84, x_85);
-if (x_77 == 0)
+lean_object* x_64; lean_object* x_65; lean_object* x_66; 
+x_64 = lean_string_append(x_60, x_63);
+lean_dec(x_63);
+x_65 = l_main_logZooms___closed__4;
+x_66 = lean_string_append(x_64, x_65);
+if (x_59 == 0)
 {
-lean_object* x_87; 
-x_87 = l_main_logZooms___closed__1;
-x_56 = x_86;
-x_57 = x_78;
-x_58 = x_80;
-x_59 = x_82;
-x_60 = x_81;
-x_61 = x_87;
-goto block_67;
+lean_object* x_67; 
+x_67 = l_main_logZooms___closed__1;
+x_47 = x_58;
+x_48 = x_66;
+x_49 = x_61;
+x_50 = x_62;
+x_51 = x_67;
+goto block_57;
 }
 else
 {
-lean_object* x_88; 
-x_88 = l_main_logZooms___closed__2;
-x_56 = x_86;
-x_57 = x_78;
-x_58 = x_80;
-x_59 = x_82;
-x_60 = x_81;
-x_61 = x_88;
-goto block_67;
+lean_object* x_68; 
+x_68 = l_main_logZooms___closed__2;
+x_47 = x_58;
+x_48 = x_66;
+x_49 = x_61;
+x_50 = x_62;
+x_51 = x_68;
+goto block_57;
 }
 }
-block_120:
+block_91:
 {
-lean_object* x_93; lean_object* x_94; lean_object* x_95; lean_object* x_96; lean_object* x_97; lean_object* x_98; lean_object* x_99; lean_object* x_100; lean_object* x_101; lean_object* x_102; lean_object* x_103; lean_object* x_104; lean_object* x_105; lean_object* x_106; lean_object* x_107; lean_object* x_108; lean_object* x_109; lean_object* x_110; lean_object* x_111; lean_object* x_112; lean_object* x_113; lean_object* x_114; lean_object* x_115; lean_object* x_116; lean_object* x_117; 
-x_93 = l_main_logZooms___closed__8;
+lean_object* x_86; lean_object* x_87; lean_object* x_88; 
+x_86 = lean_string_append(x_82, x_85);
+lean_dec(x_85);
+x_87 = l_main_logZooms___closed__7;
+x_88 = lean_string_append(x_86, x_87);
+if (x_79 == 0)
+{
+lean_object* x_89; 
+x_89 = l_main_logZooms___closed__1;
+x_58 = x_80;
+x_59 = x_81;
+x_60 = x_88;
+x_61 = x_83;
+x_62 = x_84;
+x_63 = x_89;
+goto block_69;
+}
+else
+{
+lean_object* x_90; 
+x_90 = l_main_logZooms___closed__2;
+x_58 = x_80;
+x_59 = x_81;
+x_60 = x_88;
+x_61 = x_83;
+x_62 = x_84;
+x_63 = x_90;
+goto block_69;
+}
+}
+block_122:
+{
+lean_object* x_95; lean_object* x_96; lean_object* x_97; lean_object* x_98; lean_object* x_99; lean_object* x_100; lean_object* x_101; lean_object* x_102; lean_object* x_103; lean_object* x_104; lean_object* x_105; lean_object* x_106; lean_object* x_107; lean_object* x_108; lean_object* x_109; lean_object* x_110; lean_object* x_111; lean_object* x_112; lean_object* x_113; lean_object* x_114; lean_object* x_115; lean_object* x_116; lean_object* x_117; lean_object* x_118; lean_object* x_119; 
+x_95 = l_main_logZooms___closed__8;
 lean_inc(x_8);
-x_94 = l_Nat_reprFast(x_8);
-x_95 = lean_string_append(x_93, x_94);
-lean_dec(x_94);
-x_96 = l_main_logZooms___closed__9;
+x_96 = l_Nat_reprFast(x_8);
 x_97 = lean_string_append(x_95, x_96);
-x_98 = lean_nat_add(x_8, x_25);
+lean_dec(x_96);
+x_98 = l_main_logZooms___closed__9;
+x_99 = lean_string_append(x_97, x_98);
+x_100 = lean_nat_add(x_8, x_27);
 lean_dec(x_8);
-lean_inc(x_98);
-x_99 = l_Nat_reprFast(x_98);
-x_100 = lean_string_append(x_97, x_99);
-lean_dec(x_99);
-x_101 = l_main_logZooms___closed__10;
-x_102 = lean_string_append(x_100, x_101);
-x_103 = lean_float_to_string(x_18);
+lean_inc(x_100);
+x_101 = l_Nat_reprFast(x_100);
+x_102 = lean_string_append(x_99, x_101);
+lean_dec(x_101);
+x_103 = l_main_logZooms___closed__10;
 x_104 = lean_string_append(x_102, x_103);
-lean_dec(x_103);
-x_105 = lean_string_append(x_104, x_96);
-x_106 = lean_float_to_string(x_70);
-x_107 = lean_string_append(x_105, x_106);
-lean_dec(x_106);
-x_108 = l_main_logZooms___closed__11;
+x_105 = lean_float_to_string(x_18);
+x_106 = lean_string_append(x_104, x_105);
+lean_dec(x_105);
+x_107 = lean_string_append(x_106, x_98);
+x_108 = lean_float_to_string(x_72);
 x_109 = lean_string_append(x_107, x_108);
-x_110 = lean_float_to_string(x_75);
+lean_dec(x_108);
+x_110 = l_main_logZooms___closed__11;
 x_111 = lean_string_append(x_109, x_110);
-lean_dec(x_110);
-x_112 = l_main_logZooms___closed__12;
+x_112 = lean_float_to_string(x_77);
 x_113 = lean_string_append(x_111, x_112);
-x_114 = lean_float_to_string(x_20);
+lean_dec(x_112);
+x_114 = l_main_logZooms___closed__12;
 x_115 = lean_string_append(x_113, x_114);
-lean_dec(x_114);
-x_116 = l_main_logZooms___closed__13;
+x_116 = lean_float_to_string(x_20);
 x_117 = lean_string_append(x_115, x_116);
-if (x_76 == 0)
+lean_dec(x_116);
+x_118 = l_main_logZooms___closed__13;
+x_119 = lean_string_append(x_117, x_118);
+if (x_78 == 0)
 {
-lean_object* x_118; 
-x_118 = l_main_logZooms___closed__1;
-x_78 = x_90;
-x_79 = x_117;
-x_80 = x_92;
-x_81 = x_91;
-x_82 = x_98;
-x_83 = x_118;
-goto block_89;
+lean_object* x_120; 
+x_120 = l_main_logZooms___closed__1;
+x_80 = x_94;
+x_81 = x_92;
+x_82 = x_119;
+x_83 = x_93;
+x_84 = x_100;
+x_85 = x_120;
+goto block_91;
 }
 else
 {
-lean_object* x_119; 
-x_119 = l_main_logZooms___closed__2;
-x_78 = x_90;
-x_79 = x_117;
-x_80 = x_92;
-x_81 = x_91;
-x_82 = x_98;
-x_83 = x_119;
-goto block_89;
+lean_object* x_121; 
+x_121 = l_main_logZooms___closed__2;
+x_80 = x_94;
+x_81 = x_92;
+x_82 = x_119;
+x_83 = x_93;
+x_84 = x_100;
+x_85 = x_121;
+goto block_91;
 }
 }
-block_125:
+block_127:
 {
-double x_122; double x_123; uint8_t x_124; 
-x_122 = lean_float_sub(x_70, x_18);
-x_123 = fabs(x_122);
-x_124 = lean_float_decLe(x_123, x_71);
-if (x_76 == 0)
+double x_124; double x_125; uint8_t x_126; 
+x_124 = lean_float_sub(x_72, x_18);
+x_125 = fabs(x_124);
+x_126 = lean_float_decLe(x_125, x_73);
+if (x_78 == 0)
 {
-x_90 = x_121;
-x_91 = x_124;
-x_92 = x_76;
-goto block_120;
+x_92 = x_123;
+x_93 = x_126;
+x_94 = x_78;
+goto block_122;
 }
 else
 {
-if (x_77 == 0)
+if (x_79 == 0)
 {
-x_90 = x_121;
-x_91 = x_124;
-x_92 = x_77;
-goto block_120;
+x_92 = x_123;
+x_93 = x_126;
+x_94 = x_79;
+goto block_122;
 }
 else
 {
-x_90 = x_121;
-x_91 = x_124;
-x_92 = x_124;
-goto block_120;
+x_92 = x_123;
+x_93 = x_126;
+x_94 = x_126;
+goto block_122;
 }
 }
 }
 }
 else
 {
-lean_object* x_128; lean_object* x_129; lean_object* x_130; lean_object* x_131; lean_object* x_132; lean_object* x_133; lean_object* x_134; lean_object* x_135; lean_object* x_136; lean_object* x_137; lean_object* x_138; lean_object* x_139; lean_object* x_140; lean_object* x_141; lean_object* x_142; lean_object* x_143; lean_object* x_144; lean_object* x_145; 
+lean_object* x_130; lean_object* x_131; lean_object* x_132; lean_object* x_133; lean_object* x_134; lean_object* x_135; lean_object* x_136; lean_object* x_137; lean_object* x_138; lean_object* x_139; lean_object* x_140; lean_object* x_141; lean_object* x_142; lean_object* x_143; lean_object* x_144; lean_object* x_145; lean_object* x_146; lean_object* x_147; 
 lean_dec(x_17);
 lean_dec(x_9);
 lean_dec(x_7);
 lean_dec(x_6);
 lean_dec(x_5);
 lean_dec(x_1);
-x_128 = l_main_logZooms___closed__14;
-x_129 = l_Nat_reprFast(x_8);
-x_130 = lean_string_append(x_128, x_129);
-lean_dec(x_129);
-x_131 = l_main_logZooms___closed__10;
+x_130 = l_main_logZooms___closed__14;
+x_131 = l_Nat_reprFast(x_8);
 x_132 = lean_string_append(x_130, x_131);
-x_133 = lean_float_to_string(x_18);
+lean_dec(x_131);
+x_133 = l_main_logZooms___closed__10;
 x_134 = lean_string_append(x_132, x_133);
-lean_dec(x_133);
-x_135 = l_main_logZooms___closed__12;
+x_135 = lean_float_to_string(x_18);
 x_136 = lean_string_append(x_134, x_135);
-x_137 = lean_float_to_string(x_20);
+lean_dec(x_135);
+x_137 = l_main_logZooms___closed__12;
 x_138 = lean_string_append(x_136, x_137);
-lean_dec(x_137);
-x_139 = l_main_logZooms___closed__15;
+x_139 = lean_float_to_string(x_20);
 x_140 = lean_string_append(x_138, x_139);
-x_141 = lean_float_to_string(x_2);
+lean_dec(x_139);
+x_141 = l_main_logZooms___closed__15;
 x_142 = lean_string_append(x_140, x_141);
-lean_dec(x_141);
-x_143 = l_main_logZooms___closed__16;
+x_143 = lean_float_to_string(x_2);
 x_144 = lean_string_append(x_142, x_143);
-x_145 = l_IO_println___at___main_logZooms_spec__0(x_144, x_10);
-return x_145;
+lean_dec(x_143);
+x_145 = l_main_logZooms___closed__16;
+x_146 = lean_string_append(x_144, x_145);
+x_147 = l_IO_println___at___main_logZooms_spec__0(x_146, x_10);
+return x_147;
 }
 }
 }
@@ -1886,218 +1890,227 @@ x_1 = lean_mk_string_unchecked(", safe=", 7, 7);
 return x_1;
 }
 }
-LEAN_EXPORT lean_object* l_main___lam__5(double x_1, double x_2, double x_3, lean_object* x_4, lean_object* x_5, lean_object* x_6, lean_object* x_7, lean_object* x_8, lean_object* x_9, lean_object* x_10, lean_object* x_11, double x_12, double x_13, double x_14, lean_object* x_15) {
+LEAN_EXPORT lean_object* l_main___lam__5(lean_object* x_1, uint8_t x_2, lean_object* x_3, lean_object* x_4, double x_5, double x_6, double x_7, lean_object* x_8, lean_object* x_9, lean_object* x_10, lean_object* x_11, lean_object* x_12, lean_object* x_13, lean_object* x_14, double x_15, double x_16, double x_17, lean_object* x_18) {
 _start:
 {
-lean_object* x_16; 
-x_16 = l_IO_println___at___main_logZooms_spec__0(x_11, x_15);
-if (lean_obj_tag(x_16) == 0)
+lean_object* x_19; 
+x_19 = l_IO_println___at___main_logZooms_spec__0(x_14, x_18);
+if (lean_obj_tag(x_19) == 0)
 {
-uint8_t x_17; 
-x_17 = !lean_is_exclusive(x_16);
-if (x_17 == 0)
+uint8_t x_20; 
+x_20 = !lean_is_exclusive(x_19);
+if (x_20 == 0)
 {
-lean_object* x_18; lean_object* x_19; lean_object* x_20; lean_object* x_21; lean_object* x_22; lean_object* x_23; lean_object* x_24; lean_object* x_25; lean_object* x_26; lean_object* x_27; double x_28; lean_object* x_29; double x_30; lean_object* x_31; lean_object* x_32; lean_object* x_33; lean_object* x_34; lean_object* x_35; lean_object* x_36; lean_object* x_37; lean_object* x_38; lean_object* x_39; lean_object* x_40; uint8_t x_46; 
-x_18 = lean_ctor_get(x_16, 1);
-x_19 = lean_ctor_get(x_16, 0);
+lean_object* x_21; lean_object* x_22; double x_23; lean_object* x_24; lean_object* x_25; lean_object* x_26; lean_object* x_27; lean_object* x_28; lean_object* x_29; lean_object* x_30; lean_object* x_31; lean_object* x_32; double x_33; lean_object* x_34; double x_35; lean_object* x_36; lean_object* x_37; lean_object* x_38; lean_object* x_39; lean_object* x_40; lean_object* x_41; lean_object* x_42; lean_object* x_43; lean_object* x_44; lean_object* x_45; uint8_t x_51; 
+x_21 = lean_ctor_get(x_19, 1);
+x_22 = lean_ctor_get(x_19, 0);
+lean_dec(x_22);
+x_23 = l_Float_ofScientific(x_1, x_2, x_3);
+lean_inc(x_4);
+x_24 = lean_alloc_ctor(0, 1, 16);
+lean_ctor_set(x_24, 0, x_4);
+lean_ctor_set_float(x_24, sizeof(void*)*1, x_15);
+lean_ctor_set_float(x_24, sizeof(void*)*1 + 8, x_23);
+x_25 = lean_alloc_ctor(0, 0, 24);
+lean_ctor_set_float(x_25, 0, x_5);
+lean_ctor_set_float(x_25, 8, x_6);
+lean_ctor_set_float(x_25, 16, x_6);
+x_26 = lean_alloc_ctor(0, 0, 24);
+lean_ctor_set_float(x_26, 0, x_6);
+lean_ctor_set_float(x_26, 8, x_5);
+lean_ctor_set_float(x_26, 16, x_6);
+x_27 = lean_alloc_ctor(0, 0, 24);
+lean_ctor_set_float(x_27, 0, x_6);
+lean_ctor_set_float(x_27, 8, x_6);
+lean_ctor_set_float(x_27, 16, x_5);
+x_28 = lean_box(0);
+lean_ctor_set_tag(x_19, 1);
+lean_ctor_set(x_19, 1, x_28);
+lean_ctor_set(x_19, 0, x_27);
+x_29 = lean_alloc_ctor(1, 2, 0);
+lean_ctor_set(x_29, 0, x_26);
+lean_ctor_set(x_29, 1, x_19);
+x_30 = lean_alloc_ctor(1, 2, 0);
+lean_ctor_set(x_30, 0, x_25);
+lean_ctor_set(x_30, 1, x_29);
+lean_inc(x_8);
+x_31 = lean_alloc_ctor(0, 3, 8);
+lean_ctor_set(x_31, 0, x_24);
+lean_ctor_set(x_31, 1, x_30);
+lean_ctor_set(x_31, 2, x_8);
+lean_ctor_set_float(x_31, sizeof(void*)*3, x_7);
+x_32 = l_IVI_Invariant_resonanceMatrixW(x_4, x_8);
+x_33 = l_IVI_graininessScore(x_32);
+lean_inc(x_9);
+lean_inc(x_31);
+x_34 = l_IVI_KakeyaField_withLayer(x_31, x_9);
+lean_inc(x_34);
+x_35 = l_IVI_KakeyaField_collapseScore(x_34);
+x_36 = l_main___lam__5___closed__0;
+x_37 = lean_float_to_string(x_33);
+x_38 = lean_string_append(x_36, x_37);
+lean_dec(x_37);
+x_39 = l_main_logZooms___closed__12;
+x_40 = lean_string_append(x_38, x_39);
+x_41 = lean_float_to_string(x_35);
+x_42 = lean_string_append(x_40, x_41);
+lean_dec(x_41);
+x_43 = l_main___lam__5___closed__1;
+x_44 = lean_string_append(x_42, x_43);
+x_51 = l_IVI_KakeyaField_collapseOK(x_34);
+if (x_51 == 0)
+{
+lean_object* x_52; 
+x_52 = l_main_logZooms___closed__1;
+x_45 = x_52;
+goto block_50;
+}
+else
+{
+lean_object* x_53; 
+x_53 = l_main_logZooms___closed__2;
+x_45 = x_53;
+goto block_50;
+}
+block_50:
+{
+lean_object* x_46; lean_object* x_47; 
+x_46 = lean_string_append(x_44, x_45);
+lean_dec(x_45);
+x_47 = l_IO_println___at___main_logZooms_spec__0(x_46, x_21);
+if (lean_obj_tag(x_47) == 0)
+{
+lean_object* x_48; lean_object* x_49; 
+x_48 = lean_ctor_get(x_47, 1);
+lean_inc(x_48);
+lean_dec(x_47);
+x_49 = l_main_logZooms(x_10, x_15, x_16, x_17, x_11, x_31, x_12, x_13, x_9, x_48);
+return x_49;
+}
+else
+{
+lean_dec(x_31);
+lean_dec(x_13);
+lean_dec(x_12);
+lean_dec(x_11);
+lean_dec(x_10);
+lean_dec(x_9);
+return x_47;
+}
+}
+}
+else
+{
+lean_object* x_54; double x_55; lean_object* x_56; lean_object* x_57; lean_object* x_58; lean_object* x_59; lean_object* x_60; lean_object* x_61; lean_object* x_62; lean_object* x_63; lean_object* x_64; lean_object* x_65; double x_66; lean_object* x_67; double x_68; lean_object* x_69; lean_object* x_70; lean_object* x_71; lean_object* x_72; lean_object* x_73; lean_object* x_74; lean_object* x_75; lean_object* x_76; lean_object* x_77; lean_object* x_78; uint8_t x_84; 
+x_54 = lean_ctor_get(x_19, 1);
+lean_inc(x_54);
 lean_dec(x_19);
-x_20 = lean_alloc_ctor(0, 0, 24);
-lean_ctor_set_float(x_20, 0, x_1);
-lean_ctor_set_float(x_20, 8, x_2);
-lean_ctor_set_float(x_20, 16, x_2);
-x_21 = lean_alloc_ctor(0, 0, 24);
-lean_ctor_set_float(x_21, 0, x_2);
-lean_ctor_set_float(x_21, 8, x_1);
-lean_ctor_set_float(x_21, 16, x_2);
-x_22 = lean_alloc_ctor(0, 0, 24);
-lean_ctor_set_float(x_22, 0, x_2);
-lean_ctor_set_float(x_22, 8, x_2);
-lean_ctor_set_float(x_22, 16, x_1);
-x_23 = lean_box(0);
-lean_ctor_set_tag(x_16, 1);
-lean_ctor_set(x_16, 1, x_23);
-lean_ctor_set(x_16, 0, x_22);
-x_24 = lean_alloc_ctor(1, 2, 0);
-lean_ctor_set(x_24, 0, x_21);
-lean_ctor_set(x_24, 1, x_16);
-x_25 = lean_alloc_ctor(1, 2, 0);
-lean_ctor_set(x_25, 0, x_20);
-lean_ctor_set(x_25, 1, x_24);
-lean_inc(x_5);
+x_55 = l_Float_ofScientific(x_1, x_2, x_3);
 lean_inc(x_4);
-x_26 = lean_alloc_ctor(0, 3, 16);
-lean_ctor_set(x_26, 0, x_4);
-lean_ctor_set(x_26, 1, x_25);
-lean_ctor_set(x_26, 2, x_5);
-lean_ctor_set_float(x_26, sizeof(void*)*3, x_3);
-lean_ctor_set_float(x_26, sizeof(void*)*3 + 8, x_12);
-x_27 = l_IVI_Invariant_resonanceMatrixW(x_4, x_5);
-x_28 = l_IVI_graininessScore(x_27);
-lean_inc(x_6);
-lean_inc(x_26);
-x_29 = l_IVI_KakeyaField_withLayer(x_26, x_6);
-lean_inc(x_29);
-x_30 = l_IVI_KakeyaField_collapseScore(x_29);
-x_31 = l_main___lam__5___closed__0;
-x_32 = lean_float_to_string(x_28);
-x_33 = lean_string_append(x_31, x_32);
-lean_dec(x_32);
-x_34 = l_main_logZooms___closed__12;
-x_35 = lean_string_append(x_33, x_34);
-x_36 = lean_float_to_string(x_30);
-x_37 = lean_string_append(x_35, x_36);
-lean_dec(x_36);
-x_38 = l_main___lam__5___closed__1;
-x_39 = lean_string_append(x_37, x_38);
-x_46 = l_IVI_KakeyaField_collapseOK(x_29);
-if (x_46 == 0)
+x_56 = lean_alloc_ctor(0, 1, 16);
+lean_ctor_set(x_56, 0, x_4);
+lean_ctor_set_float(x_56, sizeof(void*)*1, x_15);
+lean_ctor_set_float(x_56, sizeof(void*)*1 + 8, x_55);
+x_57 = lean_alloc_ctor(0, 0, 24);
+lean_ctor_set_float(x_57, 0, x_5);
+lean_ctor_set_float(x_57, 8, x_6);
+lean_ctor_set_float(x_57, 16, x_6);
+x_58 = lean_alloc_ctor(0, 0, 24);
+lean_ctor_set_float(x_58, 0, x_6);
+lean_ctor_set_float(x_58, 8, x_5);
+lean_ctor_set_float(x_58, 16, x_6);
+x_59 = lean_alloc_ctor(0, 0, 24);
+lean_ctor_set_float(x_59, 0, x_6);
+lean_ctor_set_float(x_59, 8, x_6);
+lean_ctor_set_float(x_59, 16, x_5);
+x_60 = lean_box(0);
+x_61 = lean_alloc_ctor(1, 2, 0);
+lean_ctor_set(x_61, 0, x_59);
+lean_ctor_set(x_61, 1, x_60);
+x_62 = lean_alloc_ctor(1, 2, 0);
+lean_ctor_set(x_62, 0, x_58);
+lean_ctor_set(x_62, 1, x_61);
+x_63 = lean_alloc_ctor(1, 2, 0);
+lean_ctor_set(x_63, 0, x_57);
+lean_ctor_set(x_63, 1, x_62);
+lean_inc(x_8);
+x_64 = lean_alloc_ctor(0, 3, 8);
+lean_ctor_set(x_64, 0, x_56);
+lean_ctor_set(x_64, 1, x_63);
+lean_ctor_set(x_64, 2, x_8);
+lean_ctor_set_float(x_64, sizeof(void*)*3, x_7);
+x_65 = l_IVI_Invariant_resonanceMatrixW(x_4, x_8);
+x_66 = l_IVI_graininessScore(x_65);
+lean_inc(x_9);
+lean_inc(x_64);
+x_67 = l_IVI_KakeyaField_withLayer(x_64, x_9);
+lean_inc(x_67);
+x_68 = l_IVI_KakeyaField_collapseScore(x_67);
+x_69 = l_main___lam__5___closed__0;
+x_70 = lean_float_to_string(x_66);
+x_71 = lean_string_append(x_69, x_70);
+lean_dec(x_70);
+x_72 = l_main_logZooms___closed__12;
+x_73 = lean_string_append(x_71, x_72);
+x_74 = lean_float_to_string(x_68);
+x_75 = lean_string_append(x_73, x_74);
+lean_dec(x_74);
+x_76 = l_main___lam__5___closed__1;
+x_77 = lean_string_append(x_75, x_76);
+x_84 = l_IVI_KakeyaField_collapseOK(x_67);
+if (x_84 == 0)
 {
-lean_object* x_47; 
-x_47 = l_main_logZooms___closed__1;
-x_40 = x_47;
-goto block_45;
+lean_object* x_85; 
+x_85 = l_main_logZooms___closed__1;
+x_78 = x_85;
+goto block_83;
 }
 else
 {
-lean_object* x_48; 
-x_48 = l_main_logZooms___closed__2;
-x_40 = x_48;
-goto block_45;
+lean_object* x_86; 
+x_86 = l_main_logZooms___closed__2;
+x_78 = x_86;
+goto block_83;
 }
-block_45:
+block_83:
 {
-lean_object* x_41; lean_object* x_42; 
-x_41 = lean_string_append(x_39, x_40);
-lean_dec(x_40);
-x_42 = l_IO_println___at___main_logZooms_spec__0(x_41, x_18);
-if (lean_obj_tag(x_42) == 0)
+lean_object* x_79; lean_object* x_80; 
+x_79 = lean_string_append(x_77, x_78);
+lean_dec(x_78);
+x_80 = l_IO_println___at___main_logZooms_spec__0(x_79, x_54);
+if (lean_obj_tag(x_80) == 0)
 {
-lean_object* x_43; lean_object* x_44; 
-x_43 = lean_ctor_get(x_42, 1);
-lean_inc(x_43);
-lean_dec(x_42);
-x_44 = l_main_logZooms(x_7, x_12, x_13, x_14, x_8, x_26, x_9, x_10, x_6, x_43);
-return x_44;
+lean_object* x_81; lean_object* x_82; 
+x_81 = lean_ctor_get(x_80, 1);
+lean_inc(x_81);
+lean_dec(x_80);
+x_82 = l_main_logZooms(x_10, x_15, x_16, x_17, x_11, x_64, x_12, x_13, x_9, x_81);
+return x_82;
 }
 else
 {
-lean_dec(x_26);
+lean_dec(x_64);
+lean_dec(x_13);
+lean_dec(x_12);
+lean_dec(x_11);
+lean_dec(x_10);
+lean_dec(x_9);
+return x_80;
+}
+}
+}
+}
+else
+{
+lean_dec(x_13);
+lean_dec(x_12);
+lean_dec(x_11);
 lean_dec(x_10);
 lean_dec(x_9);
 lean_dec(x_8);
-lean_dec(x_7);
-lean_dec(x_6);
-return x_42;
-}
-}
-}
-else
-{
-lean_object* x_49; lean_object* x_50; lean_object* x_51; lean_object* x_52; lean_object* x_53; lean_object* x_54; lean_object* x_55; lean_object* x_56; lean_object* x_57; lean_object* x_58; double x_59; lean_object* x_60; double x_61; lean_object* x_62; lean_object* x_63; lean_object* x_64; lean_object* x_65; lean_object* x_66; lean_object* x_67; lean_object* x_68; lean_object* x_69; lean_object* x_70; lean_object* x_71; uint8_t x_77; 
-x_49 = lean_ctor_get(x_16, 1);
-lean_inc(x_49);
-lean_dec(x_16);
-x_50 = lean_alloc_ctor(0, 0, 24);
-lean_ctor_set_float(x_50, 0, x_1);
-lean_ctor_set_float(x_50, 8, x_2);
-lean_ctor_set_float(x_50, 16, x_2);
-x_51 = lean_alloc_ctor(0, 0, 24);
-lean_ctor_set_float(x_51, 0, x_2);
-lean_ctor_set_float(x_51, 8, x_1);
-lean_ctor_set_float(x_51, 16, x_2);
-x_52 = lean_alloc_ctor(0, 0, 24);
-lean_ctor_set_float(x_52, 0, x_2);
-lean_ctor_set_float(x_52, 8, x_2);
-lean_ctor_set_float(x_52, 16, x_1);
-x_53 = lean_box(0);
-x_54 = lean_alloc_ctor(1, 2, 0);
-lean_ctor_set(x_54, 0, x_52);
-lean_ctor_set(x_54, 1, x_53);
-x_55 = lean_alloc_ctor(1, 2, 0);
-lean_ctor_set(x_55, 0, x_51);
-lean_ctor_set(x_55, 1, x_54);
-x_56 = lean_alloc_ctor(1, 2, 0);
-lean_ctor_set(x_56, 0, x_50);
-lean_ctor_set(x_56, 1, x_55);
-lean_inc(x_5);
-lean_inc(x_4);
-x_57 = lean_alloc_ctor(0, 3, 16);
-lean_ctor_set(x_57, 0, x_4);
-lean_ctor_set(x_57, 1, x_56);
-lean_ctor_set(x_57, 2, x_5);
-lean_ctor_set_float(x_57, sizeof(void*)*3, x_3);
-lean_ctor_set_float(x_57, sizeof(void*)*3 + 8, x_12);
-x_58 = l_IVI_Invariant_resonanceMatrixW(x_4, x_5);
-x_59 = l_IVI_graininessScore(x_58);
-lean_inc(x_6);
-lean_inc(x_57);
-x_60 = l_IVI_KakeyaField_withLayer(x_57, x_6);
-lean_inc(x_60);
-x_61 = l_IVI_KakeyaField_collapseScore(x_60);
-x_62 = l_main___lam__5___closed__0;
-x_63 = lean_float_to_string(x_59);
-x_64 = lean_string_append(x_62, x_63);
-lean_dec(x_63);
-x_65 = l_main_logZooms___closed__12;
-x_66 = lean_string_append(x_64, x_65);
-x_67 = lean_float_to_string(x_61);
-x_68 = lean_string_append(x_66, x_67);
-lean_dec(x_67);
-x_69 = l_main___lam__5___closed__1;
-x_70 = lean_string_append(x_68, x_69);
-x_77 = l_IVI_KakeyaField_collapseOK(x_60);
-if (x_77 == 0)
-{
-lean_object* x_78; 
-x_78 = l_main_logZooms___closed__1;
-x_71 = x_78;
-goto block_76;
-}
-else
-{
-lean_object* x_79; 
-x_79 = l_main_logZooms___closed__2;
-x_71 = x_79;
-goto block_76;
-}
-block_76:
-{
-lean_object* x_72; lean_object* x_73; 
-x_72 = lean_string_append(x_70, x_71);
-lean_dec(x_71);
-x_73 = l_IO_println___at___main_logZooms_spec__0(x_72, x_49);
-if (lean_obj_tag(x_73) == 0)
-{
-lean_object* x_74; lean_object* x_75; 
-x_74 = lean_ctor_get(x_73, 1);
-lean_inc(x_74);
-lean_dec(x_73);
-x_75 = l_main_logZooms(x_7, x_12, x_13, x_14, x_8, x_57, x_9, x_10, x_6, x_74);
-return x_75;
-}
-else
-{
-lean_dec(x_57);
-lean_dec(x_10);
-lean_dec(x_9);
-lean_dec(x_8);
-lean_dec(x_7);
-lean_dec(x_6);
-return x_73;
-}
-}
-}
-}
-else
-{
-lean_dec(x_10);
-lean_dec(x_9);
-lean_dec(x_8);
-lean_dec(x_7);
-lean_dec(x_6);
-lean_dec(x_5);
 lean_dec(x_4);
-return x_16;
+lean_dec(x_3);
+return x_19;
 }
 }
 }
@@ -2865,174 +2878,177 @@ x_27 = l_main___closed__6;
 x_28 = l_IO_println___at___main_logZooms_spec__0(x_27, x_26);
 if (lean_obj_tag(x_28) == 0)
 {
-lean_object* x_29; lean_object* x_30; double x_31; lean_object* x_32; double x_33; double x_34; double x_35; lean_object* x_36; lean_object* x_37; lean_object* x_38; lean_object* x_39; lean_object* x_40; lean_object* x_41; lean_object* x_42; lean_object* x_43; lean_object* x_44; lean_object* x_45; 
+lean_object* x_29; lean_object* x_30; lean_object* x_31; double x_32; lean_object* x_33; double x_34; double x_35; double x_36; lean_object* x_37; lean_object* x_38; lean_object* x_39; lean_object* x_40; lean_object* x_41; lean_object* x_42; lean_object* x_43; lean_object* x_44; lean_object* x_45; lean_object* x_46; 
 x_29 = lean_ctor_get(x_28, 1);
 lean_inc(x_29);
 lean_dec(x_28);
 x_30 = lean_unsigned_to_nat(1u);
-x_31 = l_main_logZooms___closed__5;
-x_32 = lean_unsigned_to_nat(0u);
-x_33 = l_main___closed__13;
-x_34 = l_main___closed__14;
-x_35 = l_main___closed__22;
-x_36 = lean_unsigned_to_nat(4u);
-x_37 = l_main___closed__37;
-x_38 = l_main___closed__43;
-x_39 = l_main___closed__44;
-x_40 = l_main___closed__45;
-x_41 = lean_box(0);
-x_42 = l_List_mapTR_loop___at___main_spec__13(x_39, x_41);
-x_43 = l_List_toString___at___main_spec__14(x_42);
-x_44 = lean_string_append(x_40, x_43);
-lean_dec(x_43);
-x_45 = l_IO_println___at___main_logZooms_spec__0(x_44, x_29);
-if (lean_obj_tag(x_45) == 0)
+x_31 = lean_box(1);
+x_32 = l_main_logZooms___closed__5;
+x_33 = lean_unsigned_to_nat(0u);
+x_34 = l_main___closed__13;
+x_35 = l_main___closed__14;
+x_36 = l_main___closed__22;
+x_37 = lean_unsigned_to_nat(4u);
+x_38 = l_main___closed__37;
+x_39 = l_main___closed__43;
+x_40 = l_main___closed__44;
+x_41 = l_main___closed__45;
+x_42 = lean_box(0);
+x_43 = l_List_mapTR_loop___at___main_spec__13(x_40, x_42);
+x_44 = l_List_toString___at___main_spec__14(x_43);
+x_45 = lean_string_append(x_41, x_44);
+lean_dec(x_44);
+x_46 = l_IO_println___at___main_logZooms_spec__0(x_45, x_29);
+if (lean_obj_tag(x_46) == 0)
 {
-lean_object* x_46; lean_object* x_47; lean_object* x_48; lean_object* x_49; lean_object* x_50; lean_object* x_51; lean_object* x_52; lean_object* x_53; lean_object* x_54; double x_55; lean_object* x_56; lean_object* x_57; lean_object* x_58; lean_object* x_59; lean_object* x_60; lean_object* x_61; lean_object* x_62; lean_object* x_63; lean_object* x_64; lean_object* x_65; 
-x_46 = lean_ctor_get(x_45, 1);
-lean_inc(x_46);
-lean_dec(x_45);
-x_47 = l_main___boxed__const__1;
-x_48 = l_main___boxed__const__3;
-x_49 = lean_alloc_closure((void*)(l_main___lam__0___boxed), 5, 3);
-lean_closure_set(x_49, 0, x_47);
-lean_closure_set(x_49, 1, x_38);
-lean_closure_set(x_49, 2, x_48);
-x_50 = l_main___closed__48;
-x_51 = l_IVI_Invariant_defaultWeighting;
-x_52 = l_main___closed__50;
-x_53 = l_IVI_Invariant_runUntilConverged(x_52, x_49, x_50, x_37);
-x_54 = lean_ctor_get(x_53, 0);
-lean_inc(x_54);
-x_55 = lean_ctor_get_float(x_53, sizeof(void*)*4);
-x_56 = lean_ctor_get(x_53, 1);
-lean_inc(x_56);
-x_57 = lean_ctor_get(x_53, 2);
+lean_object* x_47; lean_object* x_48; lean_object* x_49; lean_object* x_50; lean_object* x_51; lean_object* x_52; lean_object* x_53; lean_object* x_54; lean_object* x_55; double x_56; lean_object* x_57; lean_object* x_58; lean_object* x_59; lean_object* x_60; lean_object* x_61; lean_object* x_62; lean_object* x_63; lean_object* x_64; lean_object* x_65; lean_object* x_66; 
+x_47 = lean_ctor_get(x_46, 1);
+lean_inc(x_47);
+lean_dec(x_46);
+x_48 = l_main___boxed__const__1;
+x_49 = l_main___boxed__const__3;
+x_50 = lean_alloc_closure((void*)(l_main___lam__0___boxed), 5, 3);
+lean_closure_set(x_50, 0, x_48);
+lean_closure_set(x_50, 1, x_39);
+lean_closure_set(x_50, 2, x_49);
+x_51 = l_main___closed__48;
+x_52 = l_IVI_Invariant_defaultWeighting;
+x_53 = l_main___closed__50;
+x_54 = l_IVI_Invariant_runUntilConverged(x_53, x_50, x_51, x_38);
+x_55 = lean_ctor_get(x_54, 0);
+lean_inc(x_55);
+x_56 = lean_ctor_get_float(x_54, sizeof(void*)*4);
+x_57 = lean_ctor_get(x_54, 1);
 lean_inc(x_57);
-lean_dec(x_53);
-x_58 = l_main___closed__51;
-x_59 = l_Nat_reprFast(x_54);
-x_60 = lean_string_append(x_58, x_59);
-lean_dec(x_59);
-x_61 = l_main___closed__52;
-x_62 = lean_string_append(x_60, x_61);
-x_63 = lean_float_to_string(x_55);
-x_64 = lean_string_append(x_62, x_63);
-lean_dec(x_63);
-x_65 = l_IO_println___at___main_logZooms_spec__0(x_64, x_46);
-if (lean_obj_tag(x_65) == 0)
+x_58 = lean_ctor_get(x_54, 2);
+lean_inc(x_58);
+lean_dec(x_54);
+x_59 = l_main___closed__51;
+x_60 = l_Nat_reprFast(x_55);
+x_61 = lean_string_append(x_59, x_60);
+lean_dec(x_60);
+x_62 = l_main___closed__52;
+x_63 = lean_string_append(x_61, x_62);
+x_64 = lean_float_to_string(x_56);
+x_65 = lean_string_append(x_63, x_64);
+lean_dec(x_64);
+x_66 = l_IO_println___at___main_logZooms_spec__0(x_65, x_47);
+if (lean_obj_tag(x_66) == 0)
 {
-lean_object* x_66; lean_object* x_67; lean_object* x_68; lean_object* x_69; lean_object* x_70; 
-x_66 = lean_ctor_get(x_65, 1);
-lean_inc(x_66);
-lean_dec(x_65);
-x_67 = l_main___closed__53;
-x_68 = l_List_toString___at___main_spec__14(x_56);
-x_69 = lean_string_append(x_67, x_68);
-lean_dec(x_68);
-x_70 = l_IO_println___at___main_logZooms_spec__0(x_69, x_66);
-if (lean_obj_tag(x_70) == 0)
+lean_object* x_67; lean_object* x_68; lean_object* x_69; lean_object* x_70; lean_object* x_71; 
+x_67 = lean_ctor_get(x_66, 1);
+lean_inc(x_67);
+lean_dec(x_66);
+x_68 = l_main___closed__53;
+x_69 = l_List_toString___at___main_spec__14(x_57);
+x_70 = lean_string_append(x_68, x_69);
+lean_dec(x_69);
+x_71 = l_IO_println___at___main_logZooms_spec__0(x_70, x_67);
+if (lean_obj_tag(x_71) == 0)
 {
-lean_object* x_71; lean_object* x_72; lean_object* x_73; lean_object* x_74; lean_object* x_75; lean_object* x_76; 
-x_71 = lean_ctor_get(x_70, 1);
-lean_inc(x_71);
-lean_dec(x_70);
-x_72 = l_main___closed__54;
-x_73 = l_List_mapTR_loop___at___main_spec__16(x_57, x_41);
-x_74 = l_List_toString___at___main_spec__14(x_73);
-x_75 = lean_string_append(x_72, x_74);
-lean_dec(x_74);
-x_76 = l_IO_println___at___main_logZooms_spec__0(x_75, x_71);
-if (lean_obj_tag(x_76) == 0)
+lean_object* x_72; lean_object* x_73; lean_object* x_74; lean_object* x_75; lean_object* x_76; lean_object* x_77; 
+x_72 = lean_ctor_get(x_71, 1);
+lean_inc(x_72);
+lean_dec(x_71);
+x_73 = l_main___closed__54;
+x_74 = l_List_mapTR_loop___at___main_spec__16(x_58, x_42);
+x_75 = l_List_toString___at___main_spec__14(x_74);
+x_76 = lean_string_append(x_73, x_75);
+lean_dec(x_75);
+x_77 = l_IO_println___at___main_logZooms_spec__0(x_76, x_72);
+if (lean_obj_tag(x_77) == 0)
 {
-lean_object* x_77; lean_object* x_78; lean_object* x_79; lean_object* x_80; lean_object* x_81; lean_object* x_82; lean_object* x_83; lean_object* x_84; lean_object* x_85; double x_86; lean_object* x_87; 
-x_77 = lean_ctor_get(x_76, 1);
-lean_inc(x_77);
-lean_dec(x_76);
-x_78 = lean_alloc_closure((void*)(l_main___lam__1), 1, 0);
-x_79 = l_main___boxed__const__1;
-x_80 = l_main___boxed__const__2;
-x_81 = l_main___boxed__const__3;
-x_82 = lean_alloc_closure((void*)(l_main___lam__4___boxed), 10, 6);
-lean_closure_set(x_82, 0, x_79);
-lean_closure_set(x_82, 1, x_32);
-lean_closure_set(x_82, 2, x_30);
-lean_closure_set(x_82, 3, x_80);
-lean_closure_set(x_82, 4, x_78);
-lean_closure_set(x_82, 5, x_81);
-x_83 = l_main___closed__55;
-x_84 = l_main___closed__56;
-x_85 = l_main___closed__57;
-x_86 = l_main___closed__58;
-lean_inc(x_82);
-x_87 = l_main___lam__5(x_33, x_34, x_31, x_51, x_37, x_83, x_84, x_82, x_36, x_32, x_85, x_35, x_35, x_86, x_77);
-if (lean_obj_tag(x_87) == 0)
+lean_object* x_78; lean_object* x_79; lean_object* x_80; lean_object* x_81; lean_object* x_82; lean_object* x_83; lean_object* x_84; lean_object* x_85; lean_object* x_86; double x_87; uint8_t x_88; lean_object* x_89; 
+x_78 = lean_ctor_get(x_77, 1);
+lean_inc(x_78);
+lean_dec(x_77);
+x_79 = lean_alloc_closure((void*)(l_main___lam__1), 1, 0);
+x_80 = l_main___boxed__const__1;
+x_81 = l_main___boxed__const__2;
+x_82 = l_main___boxed__const__3;
+x_83 = lean_alloc_closure((void*)(l_main___lam__4___boxed), 10, 6);
+lean_closure_set(x_83, 0, x_80);
+lean_closure_set(x_83, 1, x_33);
+lean_closure_set(x_83, 2, x_30);
+lean_closure_set(x_83, 3, x_81);
+lean_closure_set(x_83, 4, x_79);
+lean_closure_set(x_83, 5, x_82);
+x_84 = l_main___closed__55;
+x_85 = l_main___closed__56;
+x_86 = l_main___closed__57;
+x_87 = l_main___closed__58;
+x_88 = lean_unbox(x_31);
+lean_inc(x_83);
+x_89 = l_main___lam__5(x_30, x_88, x_17, x_52, x_34, x_35, x_32, x_38, x_84, x_85, x_83, x_37, x_33, x_86, x_36, x_36, x_87, x_78);
+if (lean_obj_tag(x_89) == 0)
 {
-lean_object* x_88; lean_object* x_89; double x_90; lean_object* x_91; 
-x_88 = lean_ctor_get(x_87, 1);
-lean_inc(x_88);
-lean_dec(x_87);
-x_89 = l_main___closed__59;
-x_90 = l_main___closed__60;
-x_91 = l_main___lam__5(x_33, x_34, x_31, x_51, x_37, x_83, x_84, x_82, x_36, x_32, x_89, x_90, x_35, x_86, x_88);
-if (lean_obj_tag(x_91) == 0)
+lean_object* x_90; lean_object* x_91; double x_92; uint8_t x_93; lean_object* x_94; 
+x_90 = lean_ctor_get(x_89, 1);
+lean_inc(x_90);
+lean_dec(x_89);
+x_91 = l_main___closed__59;
+x_92 = l_main___closed__60;
+x_93 = lean_unbox(x_31);
+x_94 = l_main___lam__5(x_30, x_93, x_17, x_52, x_34, x_35, x_32, x_38, x_84, x_85, x_83, x_37, x_33, x_91, x_92, x_36, x_87, x_90);
+if (lean_obj_tag(x_94) == 0)
 {
-uint8_t x_92; 
-x_92 = !lean_is_exclusive(x_91);
-if (x_92 == 0)
+uint8_t x_95; 
+x_95 = !lean_is_exclusive(x_94);
+if (x_95 == 0)
 {
-lean_object* x_93; lean_object* x_94; 
-x_93 = lean_ctor_get(x_91, 0);
-lean_dec(x_93);
-x_94 = lean_box(0);
-lean_ctor_set(x_91, 0, x_94);
-return x_91;
+lean_object* x_96; lean_object* x_97; 
+x_96 = lean_ctor_get(x_94, 0);
+lean_dec(x_96);
+x_97 = lean_box(0);
+lean_ctor_set(x_94, 0, x_97);
+return x_94;
 }
 else
 {
-lean_object* x_95; lean_object* x_96; lean_object* x_97; 
-x_95 = lean_ctor_get(x_91, 1);
-lean_inc(x_95);
-lean_dec(x_91);
-x_96 = lean_box(0);
-x_97 = lean_alloc_ctor(0, 2, 0);
-lean_ctor_set(x_97, 0, x_96);
-lean_ctor_set(x_97, 1, x_95);
-return x_97;
-}
-}
-else
-{
-return x_91;
-}
-}
-else
-{
-lean_dec(x_82);
-return x_87;
+lean_object* x_98; lean_object* x_99; lean_object* x_100; 
+x_98 = lean_ctor_get(x_94, 1);
+lean_inc(x_98);
+lean_dec(x_94);
+x_99 = lean_box(0);
+x_100 = lean_alloc_ctor(0, 2, 0);
+lean_ctor_set(x_100, 0, x_99);
+lean_ctor_set(x_100, 1, x_98);
+return x_100;
 }
 }
 else
 {
-return x_76;
+return x_94;
 }
 }
 else
 {
+lean_dec(x_83);
+return x_89;
+}
+}
+else
+{
+return x_77;
+}
+}
+else
+{
+lean_dec(x_58);
+return x_71;
+}
+}
+else
+{
+lean_dec(x_58);
 lean_dec(x_57);
-return x_70;
+return x_66;
 }
 }
 else
 {
-lean_dec(x_57);
-lean_dec(x_56);
-return x_65;
-}
-}
-else
-{
-return x_45;
+return x_46;
 }
 }
 else
@@ -3220,24 +3236,45 @@ x_17 = lean_box_float(x_16);
 return x_17;
 }
 }
-LEAN_EXPORT lean_object* l_main___lam__5___boxed(lean_object* x_1, lean_object* x_2, lean_object* x_3, lean_object* x_4, lean_object* x_5, lean_object* x_6, lean_object* x_7, lean_object* x_8, lean_object* x_9, lean_object* x_10, lean_object* x_11, lean_object* x_12, lean_object* x_13, lean_object* x_14, lean_object* x_15) {
+LEAN_EXPORT lean_object* l_main___lam__5___boxed(lean_object** _args) {
+lean_object* x_1 = _args[0];
+lean_object* x_2 = _args[1];
+lean_object* x_3 = _args[2];
+lean_object* x_4 = _args[3];
+lean_object* x_5 = _args[4];
+lean_object* x_6 = _args[5];
+lean_object* x_7 = _args[6];
+lean_object* x_8 = _args[7];
+lean_object* x_9 = _args[8];
+lean_object* x_10 = _args[9];
+lean_object* x_11 = _args[10];
+lean_object* x_12 = _args[11];
+lean_object* x_13 = _args[12];
+lean_object* x_14 = _args[13];
+lean_object* x_15 = _args[14];
+lean_object* x_16 = _args[15];
+lean_object* x_17 = _args[16];
+lean_object* x_18 = _args[17];
 _start:
 {
-double x_16; double x_17; double x_18; double x_19; double x_20; double x_21; lean_object* x_22; 
-x_16 = lean_unbox_float(x_1);
-lean_dec(x_1);
-x_17 = lean_unbox_float(x_2);
+uint8_t x_19; double x_20; double x_21; double x_22; double x_23; double x_24; double x_25; lean_object* x_26; 
+x_19 = lean_unbox(x_2);
 lean_dec(x_2);
-x_18 = lean_unbox_float(x_3);
-lean_dec(x_3);
-x_19 = lean_unbox_float(x_12);
-lean_dec(x_12);
-x_20 = lean_unbox_float(x_13);
-lean_dec(x_13);
-x_21 = lean_unbox_float(x_14);
-lean_dec(x_14);
-x_22 = l_main___lam__5(x_16, x_17, x_18, x_4, x_5, x_6, x_7, x_8, x_9, x_10, x_11, x_19, x_20, x_21, x_15);
-return x_22;
+x_20 = lean_unbox_float(x_5);
+lean_dec(x_5);
+x_21 = lean_unbox_float(x_6);
+lean_dec(x_6);
+x_22 = lean_unbox_float(x_7);
+lean_dec(x_7);
+x_23 = lean_unbox_float(x_15);
+lean_dec(x_15);
+x_24 = lean_unbox_float(x_16);
+lean_dec(x_16);
+x_25 = lean_unbox_float(x_17);
+lean_dec(x_17);
+x_26 = l_main___lam__5(x_1, x_19, x_3, x_4, x_20, x_21, x_22, x_8, x_9, x_10, x_11, x_12, x_13, x_14, x_23, x_24, x_25, x_18);
+lean_dec(x_1);
+return x_26;
 }
 }
 lean_object* initialize_Init(uint8_t builtin, lean_object*);
