.lake/build/ir/IVI/Kakeya.c
@@ -1,6 +1,6 @@
 // Lean compiler output
 // Module: IVI.Kakeya
-// Imports: Init IVI.Intangible IVI.Invariant IVI.Harmonics IVI.SchematismEvidence
+// Imports: Init IVI.Intangible IVI.Invariant IVI.Harmonics IVI.Collapse IVI.SchematismEvidence
 #include <lean/lean.h>
 #if defined(__clang__)
 #pragma clang diagnostic ignored "-Wunused-parameter"
@@ -13,10 +13,12 @@
 #ifdef __cplusplus
 extern "C" {
 #endif
+uint8_t l_IVI_ICollapseCfg_grainSafeBool(lean_object*, lean_object*);
 lean_object* l_Float_repr(double, lean_object*);
 static lean_object* l_IVI_reprDir3___redArg___closed__13____x40_IVI_Kakeya___hyg_41_;
 double lean_float_mul(double, double);
 LEAN_EXPORT uint8_t l_IVI_realizes(double, lean_object*, lean_object*);
+LEAN_EXPORT lean_object* l___private_IVI_Kakeya_0__IVI_spectralGraininess_match__1_splitter(lean_object*, lean_object*, lean_object*, lean_object*);
 LEAN_EXPORT lean_object* l_IVI_invariantFromKakeya___boxed(lean_object*, lean_object*, lean_object*, lean_object*, lean_object*, lean_object*, lean_object*);
 double lean_float_div(double, double);
 static lean_object* l_IVI_reprDir3___redArg___closed__7____x40_IVI_Kakeya___hyg_41_;
@@ -25,20 +27,26 @@ lean_object* l_IVI_Intangible_normaliseDir(lean_object*);
 LEAN_EXPORT double l_IVI_KakeyaField_collapseScore(lean_object*);
 LEAN_EXPORT double l_IVI_dirDot(lean_object*, lean_object*);
 static lean_object* l_IVI_reprDir3___redArg___closed__9____x40_IVI_Kakeya___hyg_41_;
-uint8_t lean_float_decLt(double, double);
 LEAN_EXPORT lean_object* l_IVI_KakeyaField_collapseOK___boxed(lean_object*);
 static lean_object* l_IVI_reprDir3___redArg___closed__3____x40_IVI_Kakeya___hyg_41_;
+LEAN_EXPORT lean_object* l_IVI_KakeyaField_weighting(lean_object*);
 LEAN_EXPORT uint8_t l_IVI_KakeyaField_collapseOK(lean_object*);
+LEAN_EXPORT lean_object* l___private_IVI_Kakeya_0__IVI_harmonicSummary_match__1_splitter___redArg(lean_object*, lean_object*, lean_object*);
+LEAN_EXPORT lean_object* l_IVI_KakeyaField_weighting___boxed(lean_object*);
+uint8_t l_IVI_ICollapseCfg_grainCollapseBool(lean_object*, lean_object*);
 LEAN_EXPORT lean_object* l_IVI_invariantFromKakeya(lean_object*, uint8_t, double, double, lean_object*, lean_object*, lean_object*);
-double l_IVI_graininessScore(lean_object*);
 double sqrt(double);
 LEAN_EXPORT lean_object* l_IVI_KakeyaField_collapseScore___boxed(lean_object*);
 double lean_float_add(double, double);
 lean_object* lean_nat_to_int(lean_object*);
+LEAN_EXPORT lean_object* l___private_IVI_Kakeya_0__IVI_spectralGraininess_match__1_splitter___boxed(lean_object*, lean_object*, lean_object*, lean_object*);
 static lean_object* l_IVI_reprDir3___redArg___closed__2____x40_IVI_Kakeya___hyg_41_;
+LEAN_EXPORT lean_object* l___private_IVI_Kakeya_0__IVI_spectralGraininess_match__1_splitter___redArg___boxed(lean_object*, lean_object*, lean_object*);
 LEAN_EXPORT lean_object* l_IVI_KakeyaField_collapseExceededBool___boxed(lean_object*);
 LEAN_EXPORT lean_object* l_IVI_reprDir3____x40_IVI_Kakeya___hyg_41_(lean_object*, lean_object*);
 LEAN_EXPORT lean_object* l_IVI_reprDir3___redArg____x40_IVI_Kakeya___hyg_41_(lean_object*);
+LEAN_EXPORT lean_object* l___private_IVI_Kakeya_0__IVI_harmonicSummary_match__1_splitter___redArg___boxed(lean_object*, lean_object*, lean_object*);
+LEAN_EXPORT lean_object* l___private_IVI_Kakeya_0__IVI_harmonicSummary_match__1_splitter___boxed(lean_object*, lean_object*, lean_object*, lean_object*);
 static double l_IVI_normaliseDir3___closed__1;
 static double l_IVI_normaliseDir3___closed__0;
 static lean_object* l_IVI_instReprDir3___closed__0;
@@ -55,10 +63,12 @@ static lean_object* l_IVI_reprDir3___redArg___closed__11____x40_IVI_Kakeya___hyg
 static lean_object* l_IVI_reprDir3___redArg___closed__0____x40_IVI_Kakeya___hyg_41_;
 uint8_t lean_float_decLe(double, double);
 LEAN_EXPORT uint8_t l_IVI_KakeyaField_collapseExceededBool(lean_object*);
+LEAN_EXPORT lean_object* l___private_IVI_Kakeya_0__IVI_harmonicSummary_match__1_splitter(lean_object*, lean_object*, lean_object*, lean_object*);
 static lean_object* l_IVI_reprDir3___redArg___closed__15____x40_IVI_Kakeya___hyg_41_;
 static lean_object* l_IVI_reprDir3___redArg___closed__6____x40_IVI_Kakeya___hyg_41_;
 LEAN_EXPORT lean_object* l_IVI_instReprDir3;
 static lean_object* l_IVI_reprDir3___redArg___closed__14____x40_IVI_Kakeya___hyg_41_;
+double l_IVI_ICollapseCfg_collapseScore(lean_object*, lean_object*);
 LEAN_EXPORT lean_object* l_IVI_dirDot___boxed(lean_object*, lean_object*);
 static lean_object* l_IVI_reprDir3___redArg___closed__4____x40_IVI_Kakeya___hyg_41_;
 LEAN_EXPORT lean_object* l_IVI_normaliseDir3(lean_object*);
@@ -66,8 +76,8 @@ LEAN_EXPORT lean_object* l_IVI_reprDir3____x40_IVI_Kakeya___hyg_41____boxed(lean
 LEAN_EXPORT lean_object* l_IVI_KakeyaField_withNodes(lean_object*, lean_object*);
 static lean_object* l_IVI_normaliseDir3___closed__2;
 static lean_object* l_IVI_reprDir3___redArg___closed__17____x40_IVI_Kakeya___hyg_41_;
+LEAN_EXPORT lean_object* l___private_IVI_Kakeya_0__IVI_spectralGraininess_match__1_splitter___redArg(lean_object*, lean_object*, lean_object*);
 static lean_object* l_IVI_reprDir3___redArg___closed__12____x40_IVI_Kakeya___hyg_41_;
-lean_object* l_IVI_Invariant_resonanceMatrixW(lean_object*, lean_object*);
 LEAN_EXPORT lean_object* l_IVI_reprDir3___redArg____x40_IVI_Kakeya___hyg_41____boxed(lean_object*);
 double lean_float_sub(double, double);
 static lean_object* l_IVI_reprDir3___redArg___closed__10____x40_IVI_Kakeya___hyg_41_;
@@ -565,18 +575,36 @@ x_6 = lean_box(x_5);
 return x_6;
 }
 }
+LEAN_EXPORT lean_object* l_IVI_KakeyaField_weighting(lean_object* x_1) {
+_start:
+{
+lean_object* x_2; lean_object* x_3; 
+x_2 = lean_ctor_get(x_1, 0);
+x_3 = lean_ctor_get(x_2, 0);
+lean_inc(x_3);
+return x_3;
+}
+}
+LEAN_EXPORT lean_object* l_IVI_KakeyaField_weighting___boxed(lean_object* x_1) {
+_start:
+{
+lean_object* x_2; 
+x_2 = l_IVI_KakeyaField_weighting(x_1);
+lean_dec(x_1);
+return x_2;
+}
+}
 LEAN_EXPORT double l_IVI_KakeyaField_collapseScore(lean_object* x_1) {
 _start:
 {
-lean_object* x_2; lean_object* x_3; lean_object* x_4; double x_5; 
+lean_object* x_2; lean_object* x_3; double x_4; 
 x_2 = lean_ctor_get(x_1, 0);
 lean_inc(x_2);
 x_3 = lean_ctor_get(x_1, 2);
 lean_inc(x_3);
 lean_dec(x_1);
-x_4 = l_IVI_Invariant_resonanceMatrixW(x_2, x_3);
-x_5 = l_IVI_graininessScore(x_4);
-return x_5;
+x_4 = l_IVI_ICollapseCfg_collapseScore(x_2, x_3);
+return x_4;
 }
 }
 LEAN_EXPORT lean_object* l_IVI_KakeyaField_collapseScore___boxed(lean_object* x_1) {
@@ -591,10 +619,13 @@ return x_3;
 LEAN_EXPORT uint8_t l_IVI_KakeyaField_collapseOK(lean_object* x_1) {
 _start:
 {
-double x_2; double x_3; uint8_t x_4; 
-x_2 = lean_ctor_get_float(x_1, sizeof(void*)*3 + 8);
-x_3 = l_IVI_KakeyaField_collapseScore(x_1);
-x_4 = lean_float_decLe(x_3, x_2);
+lean_object* x_2; lean_object* x_3; uint8_t x_4; 
+x_2 = lean_ctor_get(x_1, 0);
+lean_inc(x_2);
+x_3 = lean_ctor_get(x_1, 2);
+lean_inc(x_3);
+lean_dec(x_1);
+x_4 = l_IVI_ICollapseCfg_grainSafeBool(x_2, x_3);
 return x_4;
 }
 }
@@ -610,10 +641,13 @@ return x_3;
 LEAN_EXPORT uint8_t l_IVI_KakeyaField_collapseExceededBool(lean_object* x_1) {
 _start:
 {
-double x_2; double x_3; uint8_t x_4; 
-x_2 = lean_ctor_get_float(x_1, sizeof(void*)*3 + 8);
-x_3 = l_IVI_KakeyaField_collapseScore(x_1);
-x_4 = lean_float_decLt(x_2, x_3);
+lean_object* x_2; lean_object* x_3; uint8_t x_4; 
+x_2 = lean_ctor_get(x_1, 0);
+lean_inc(x_2);
+x_3 = lean_ctor_get(x_1, 2);
+lean_inc(x_3);
+lean_dec(x_1);
+x_4 = l_IVI_ICollapseCfg_grainCollapseBool(x_2, x_3);
 return x_4;
 }
 }
@@ -624,6 +658,97 @@ uint8_t x_2; lean_object* x_3;
 x_2 = l_IVI_KakeyaField_collapseExceededBool(x_1);
 x_3 = lean_box(x_2);
 return x_3;
+}
+}
+LEAN_EXPORT lean_object* l___private_IVI_Kakeya_0__IVI_harmonicSummary_match__1_splitter___redArg(lean_object* x_1, lean_object* x_2, lean_object* x_3) {
+_start:
+{
+if (lean_obj_tag(x_1) == 0)
+{
+lean_dec(x_3);
+lean_inc(x_2);
+return x_2;
+}
+else
+{
+lean_object* x_4; lean_object* x_5; lean_object* x_6; 
+x_4 = lean_ctor_get(x_1, 0);
+lean_inc(x_4);
+x_5 = lean_ctor_get(x_1, 1);
+lean_inc(x_5);
+lean_dec(x_1);
+x_6 = lean_apply_2(x_3, x_4, x_5);
+return x_6;
+}
+}
+}
+LEAN_EXPORT lean_object* l___private_IVI_Kakeya_0__IVI_harmonicSummary_match__1_splitter(lean_object* x_1, lean_object* x_2, lean_object* x_3, lean_object* x_4) {
+_start:
+{
+lean_object* x_5; 
+x_5 = l___private_IVI_Kakeya_0__IVI_harmonicSummary_match__1_splitter___redArg(x_2, x_3, x_4);
+return x_5;
+}
+}
+LEAN_EXPORT lean_object* l___private_IVI_Kakeya_0__IVI_harmonicSummary_match__1_splitter___redArg___boxed(lean_object* x_1, lean_object* x_2, lean_object* x_3) {
+_start:
+{
+lean_object* x_4; 
+x_4 = l___private_IVI_Kakeya_0__IVI_harmonicSummary_match__1_splitter___redArg(x_1, x_2, x_3);
+lean_dec(x_2);
+return x_4;
+}
+}
+LEAN_EXPORT lean_object* l___private_IVI_Kakeya_0__IVI_harmonicSummary_match__1_splitter___boxed(lean_object* x_1, lean_object* x_2, lean_object* x_3, lean_object* x_4) {
+_start:
+{
+lean_object* x_5; 
+x_5 = l___private_IVI_Kakeya_0__IVI_harmonicSummary_match__1_splitter(x_1, x_2, x_3, x_4);
+lean_dec(x_3);
+return x_5;
+}
+}
+LEAN_EXPORT lean_object* l___private_IVI_Kakeya_0__IVI_spectralGraininess_match__1_splitter___redArg(lean_object* x_1, lean_object* x_2, lean_object* x_3) {
+_start:
+{
+if (lean_obj_tag(x_1) == 0)
+{
+lean_dec(x_3);
+lean_inc(x_2);
+return x_2;
+}
+else
+{
+lean_object* x_4; 
+x_4 = lean_apply_2(x_3, x_1, lean_box(0));
+return x_4;
+}
+}
+}
+LEAN_EXPORT lean_object* l___private_IVI_Kakeya_0__IVI_spectralGraininess_match__1_splitter(lean_object* x_1, lean_object* x_2, lean_object* x_3, lean_object* x_4) {
+_start:
+{
+lean_object* x_5; 
+x_5 = l___private_IVI_Kakeya_0__IVI_spectralGraininess_match__1_splitter___redArg(x_2, x_3, x_4);
+return x_5;
+}
+}
+LEAN_EXPORT lean_object* l___private_IVI_Kakeya_0__IVI_spectralGraininess_match__1_splitter___redArg___boxed(lean_object* x_1, lean_object* x_2, lean_object* x_3) {
+_start:
+{
+lean_object* x_4; 
+x_4 = l___private_IVI_Kakeya_0__IVI_spectralGraininess_match__1_splitter___redArg(x_1, x_2, x_3);
+lean_dec(x_2);
+return x_4;
+}
+}
+LEAN_EXPORT lean_object* l___private_IVI_Kakeya_0__IVI_spectralGraininess_match__1_splitter___boxed(lean_object* x_1, lean_object* x_2, lean_object* x_3, lean_object* x_4) {
+_start:
+{
+lean_object* x_5; 
+x_5 = l___private_IVI_Kakeya_0__IVI_spectralGraininess_match__1_splitter(x_1, x_2, x_3, x_4);
+lean_dec(x_3);
+return x_5;
 }
 }
 LEAN_EXPORT lean_object* l_IVI_KakeyaField_withNodes(lean_object* x_1, lean_object* x_2) {
@@ -641,21 +766,19 @@ return x_1;
 }
 else
 {
-double x_5; double x_6; lean_object* x_7; lean_object* x_8; lean_object* x_9; 
+double x_5; lean_object* x_6; lean_object* x_7; lean_object* x_8; 
 x_5 = lean_ctor_get_float(x_1, sizeof(void*)*3);
-x_6 = lean_ctor_get_float(x_1, sizeof(void*)*3 + 8);
-x_7 = lean_ctor_get(x_1, 0);
-x_8 = lean_ctor_get(x_1, 1);
-lean_inc(x_8);
+x_6 = lean_ctor_get(x_1, 0);
+x_7 = lean_ctor_get(x_1, 1);
 lean_inc(x_7);
+lean_inc(x_6);
 lean_dec(x_1);
-x_9 = lean_alloc_ctor(0, 3, 16);
-lean_ctor_set(x_9, 0, x_7);
-lean_ctor_set(x_9, 1, x_8);
-lean_ctor_set(x_9, 2, x_2);
-lean_ctor_set_float(x_9, sizeof(void*)*3, x_5);
-lean_ctor_set_float(x_9, sizeof(void*)*3 + 8, x_6);
-return x_9;
+x_8 = lean_alloc_ctor(0, 3, 8);
+lean_ctor_set(x_8, 0, x_6);
+lean_ctor_set(x_8, 1, x_7);
+lean_ctor_set(x_8, 2, x_2);
+lean_ctor_set_float(x_8, sizeof(void*)*3, x_5);
+return x_8;
 }
 }
 }
@@ -689,6 +812,7 @@ lean_object* initialize_Init(uint8_t builtin, lean_object*);
 lean_object* initialize_IVI_Intangible(uint8_t builtin, lean_object*);
 lean_object* initialize_IVI_Invariant(uint8_t builtin, lean_object*);
 lean_object* initialize_IVI_Harmonics(uint8_t builtin, lean_object*);
+lean_object* initialize_IVI_Collapse(uint8_t builtin, lean_object*);
 lean_object* initialize_IVI_SchematismEvidence(uint8_t builtin, lean_object*);
 static bool _G_initialized = false;
 LEAN_EXPORT lean_object* initialize_IVI_Kakeya(uint8_t builtin, lean_object* w) {
@@ -705,6 +829,9 @@ res = initialize_IVI_Invariant(builtin, lean_io_mk_world());
 if (lean_io_result_is_error(res)) return res;
 lean_dec_ref(res);
 res = initialize_IVI_Harmonics(builtin, lean_io_mk_world());
+if (lean_io_result_is_error(res)) return res;
+lean_dec_ref(res);
+res = initialize_IVI_Collapse(builtin, lean_io_mk_world());
 if (lean_io_result_is_error(res)) return res;
 lean_dec_ref(res);
 res = initialize_IVI_SchematismEvidence(builtin, lean_io_mk_world());
